{"cells":[{"cell_type":"markdown","metadata":{"id":"lJCEyyf3IlRw"},"source":["# HW1 - Q1: Linear Algebra Basics (30 points)\n","Notes:\n","* Questions (a), (b), (c), and (d) need to be typewritten.\n","* Important:\n","  * Write all the steps of the solution. \n","  * Use proper LATEX formatting and notation for all mathematical equations, vectors, and matrices. \n"]},{"cell_type":"markdown","metadata":{"id":"Cdpgzds_Isxc"},"source":["### **(a)** Given $L_1$ and $L_2$ are two lower triangular matrices of size $n\\times n$, prove that $L_1L_2$ is also a lower triangular matrix. Further, prove by induction that multiplication of $m\\,(m>2)$ lower triangular matrices ($L_1, L_2,..., L_m$) is also a lower triangular matrix. (6 points)"]},{"cell_type":"markdown","metadata":{"id":"i_qPxVfOI34J"},"source":["#### <font color=\"red\">Your answer here:</font>"]},{"cell_type":"markdown","metadata":{"id":"FnMgRMp64_ab"},"source":["\n","\n","---\n","\n","\n"]},{"cell_type":"markdown","metadata":{"id":"nEj1Gbc2JDn8"},"source":["### **(b)** Use Gauss elimination to solve the following equations: (8 points)\n","$-4x_1 + 5x_2 - 5x_3 = -29$\\\n","$-8x_1  -5x_2 - 3x_3 = -15$\\\n","$16x_1 - 5x_2 + 6x_3 = 45$"]},{"cell_type":"markdown","metadata":{"id":"4F8bIVBhJY1A"},"source":["#### <font color=\"red\">Your answer here:</font>\n","\n","**Gaussian elimitation**:  \n","\n","$\\begin{bmatrix} -4 & 5 & -5 \\\\ -8 & -5 & -3 \\\\ 16 & -5 & 6 \\end{bmatrix}$\n","$\\begin{bmatrix} -29 \\\\ -15 \\\\ 45 \\end{bmatrix}$\n","$\\begin{matrix} -\\mathbf{L_1}- \\\\ row2 - 2row1\\\\ row3 - 4row1 \\end{matrix}$\n","$\\begin{bmatrix} -4 & 5 & -5 \\\\ 0 & -15 & 7 \\\\ 0 & 15 & -14 \\end{bmatrix}$\n","$\\begin{bmatrix} -29 \\\\ 43 \\\\ -71 \\end{bmatrix}$\n","$\\begin{matrix} -\\mathbf{L_2}- \\\\ \\\\ row3 + row2 \\end{matrix}$\n","$\\begin{bmatrix} -4 & 5 & -5 \\\\ 0 & -15 & 7 \\\\ 0 & 0 & -7 \\end{bmatrix}$\n","$\\begin{bmatrix} -29 \\\\ 43 \\\\ -28 \\end{bmatrix}$  \n","\n","**backward substitution**:  \n","\n","step3: $-4x_1 + 5x_2 - 5x_3 = -29 \\implies -4x_1 + 5(-1) - 5(4) = -29 \\implies \\mathbf{x_1 = 1}$  \n","step2: $-15x_2 + 7x_3 = 43 \\implies -15x_2 + 7(4) = 43 \\implies \\mathbf{x_2=-1}$  \n","step1: $-7x_3 = -28 \\implies \\mathbf{x_3=4}$  \n","\n","**solution**:  \n","\n","$\\begin{bmatrix} x_1 \\\\ x_2 \\\\ x_3 \\end{bmatrix} = \\begin{bmatrix} 1 \\\\ -1 \\\\ 4 \\end{bmatrix}$"]},{"cell_type":"markdown","metadata":{"id":"vO1TrTMH5BhT"},"source":["\n","\n","---\n"]},{"cell_type":"markdown","metadata":{"id":"kKI0kyPGJdgh"},"source":["### **(c)** Do the $LU$ decomposition for the matrix obtained in (b). Using the matrices $L$ and $U$, do forward and backward substitution and solve for $\\mathbf{x}$. Match your answer with the solution obtained in (b). (8 points)"]},{"cell_type":"markdown","metadata":{"id":"e4ytt-NSJla9"},"source":["#### <font color=\"red\">Your answer here:</font>\n","\n","From the matrices obtained in *Q1 (b)*, we can decompose $\\mathbf{A=LU}$ given:  \n","\n","$\\mathbf{A} = \\begin{bmatrix} -4 & 5 & -5 \\\\ -8 & -5 & -3 \\\\ 16 & -5 & 6 \\end{bmatrix}$, \n","$\\mathbf{U} = \\begin{bmatrix} -4 & 5 & -5 \\\\ 0 & -15 & 7 \\\\ 0 & 0 & -7 \\end{bmatrix}$,\n","$\\underbrace{\\mathbf{L}}_{L_2(L_1A)} = \\begin{bmatrix} 1 & 0 & 0 \\\\ 2 & 1 & 0 \\\\ -4 & -1 & 1 \\end{bmatrix}$  \n","\n","**solve for $\\mathbf{y}$**  \n","\n","Since $\\mathbf{Ax = b \\implies L\\underbrace{Ux}_y = b \\implies Ly = b}$, $\\mathbf{y}$ can be solved by forward substitution:  \n","\n","step1: $\\mathbf{y_1 = -29}$  \n","step2: $2y_1 + y_2 = -15 \\implies 2(-29) + y_2 = -15 \\implies \\mathbf{y_2 = 43}$  \n","step3: $-4y_1 -y_2 + y_3 = 45 \\implies -4(-29) -43 + y_3 = 45 \\implies \\mathbf{y_3 = -28}$  \n","\n","$\\begin{bmatrix} y_1 \\\\ y_2 \\\\ y_3 \\end{bmatrix} = \\begin{bmatrix} -29 \\\\ 43 \\\\ -28 \\end{bmatrix}$\n","\n","**solve for $\\mathbf{x}$**  \n","\n","Since $\\mathbf{Ux = y}$, $\\mathbf{x}$ can be solved by backward substitution:  \n","\n","step3: $-4x_1 + 5x_2 -5x_3 = -29 \\implies -4x_1 + 5(-1) - 5(4) = -29 \\implies \\mathbf{x_1 = 1}$  \n","step2: $-15x_2 + 7x_3 = 43 \\implies -15x_2 + 7(4) = 43 \\implies \\mathbf{x_2 = -1}$  \n","step1: $-7x_3 = -28 \\implies \\mathbf{x_3 = 4}$\n","\n","**solution**:  \n","\n","$\\begin{bmatrix} x_1 \\\\ x_2 \\\\ x_3 \\end{bmatrix} = \\begin{bmatrix} 1 \\\\ -1 \\\\ 4 \\end{bmatrix}$"]},{"cell_type":"markdown","metadata":{"id":"3mGCqU7N5FkL"},"source":["\n","\n","---\n","\n"]},{"cell_type":"markdown","metadata":{"id":"Lj8zlLl6Jl7D"},"source":["### **(d)** Do the $QR$ decomposition for the matrix obtained in (b) using Gram-Schmidt algorithm. Using the decomposition, solve for $\\mathbf{x}$. Match your answer with the solution obtained in problem (b). (8 points)"]},{"cell_type":"markdown","metadata":{"id":"7E4qy1MTJsJ8"},"source":["#### <font color=\"red\">Your answer here:</font>"]},{"cell_type":"markdown","metadata":{"id":"SsvvDcejL3CH"},"source":["\n","\n","---\n","\n"]}],"metadata":{"colab":{"collapsed_sections":[],"provenance":[]},"kernelspec":{"display_name":"Python 3.8.9 64-bit","language":"python","name":"python3"},"language_info":{"name":"python","version":"3.8.9"},"vscode":{"interpreter":{"hash":"31f2aee4e71d21fbe5cf8b01ff0e069b9275f58929596ceb00d14d90e3e16cd6"}}},"nbformat":4,"nbformat_minor":0}
